<?xml version="1.0" encoding="UTF-8"?>
<section xml:id="s-Systems-of-Equations">
	<title>Systems of Equations</title>
	<idx>Systems of Equations</idx>

	<introduction>
		<p>In this section we will learn how to solve multiple linear equations with multiple unknowns using matrices.</p>
	</introduction>
	<subsection xml:id="ss-elementary-operations">
		<title>Elementary Operations</title>
        <p>
            Consider the following example.
        </p>
        <example><title>Solution Set</title>
            <idx>Solution Set</idx>
            <p>
                Find <m>x</m> and <m>y</m> such that
                <me>x + y = 7 \text{ and } 2x - y = 8.</me>
            </p>
            <p>
                The set of ordered pairs, (x, y) which solve both equations is called the <term>solution set</term>.
            </p>
            <p>
                You can verify that <m>(x, y) = (5, 2)</m> is a solution to the above system. The interesting
                question is this: If you were not given this information to verify, how could you determine
                the solution? You can do this by using the following basic operations on the equations,
                none of which change the set of solutions of the system of equations. 
            </p>
        </example>

		<definition xml:id="def-elementary-operations">
			<title>Elementary Operations</title>
			<idx>Elementary Operations</idx>
			<statement>
				<p><term>Elementary operations</term> are those operations consisting of the following.
                    <ol>
                        <li>
                            <p>
                                Interchange the order in which the equations are listed.  
                            </p>
                        </li>
                        <li>
                            <p>
                                Multiply any equation by a nonzero number. 
                            </p>
                        </li>
                        <li>
                            <p>
                                Replace any equation with itself added to a multiple of another equation.
                            </p>
                        </li>
                    </ol></p>
			</statement>
		</definition>


		<example xml:id="ex-some-elementary-operations">

			<p> To illustrate the third of these operations on this particular system, consider the following.
                <me>x + y = 7</me>
                <me>2x - y = 8</me>
                The system has the same solution set as the system
                <me>x + y = 7</me>
                <me>-3y = -6.</me>
                To obtain the second system, take the second equation of the first system and add <m>-2</m> times the first equation to obtain
<m>-3y = -6</m>. Now, this clearly shows that <m>y = 2</m> and so it follows from the other equation that <m>x + 2 = 7</m>
and so <m>x = 5</m>.
            </p>
		</example>

		

		<p> Of course a linear system may involve many equations and many variables. The so-
            lution set is still the collection of solutions to the equations. In every case, the above
            operations of <xref ref="def-elementary-operations"/> do not change the set of solutions to the system of linear
            equations.</p>

            <theorem xml:id="thm-elementary-operations">
                <statement>
                    <p>
                        Suppose you have two equations, involving the variables,
                        <m>(x_1 , · · · , x_n )</m>
                        <me>E_1 = f_1 , E_2 = f_2</me>
                        where <m>E_1</m> and <m>E_2</m> are expressions involving the variables and <m>f_1</m> and <m>f_2</m> are constants. (In
                        the above example there are only two variables, <m>x</m> and <m>y</m> and <m>E_1 = x + y</m> while <m>E_2 = 2x - y</m>.)
                        Then the system <m>E_1 = f_1, E_2 = f_2</m> has the same solution set as
                       <me> E_1 = f_1, E_2 + aE_1 = f_2 + a f_1</me> 
                        Also the system <m>E_1 = f_1 , E_2 = f_2</m> has the same solutions as the system, <m>E_2 = f_2 , E_1 = f_1</m>. The
                        system <m>E_1 = f_1 , E_2 = f_2</m> has the same solution as the system <m>E_1 = f_1, aE_2 = a f_2</m> provided
                        <m>a \neq 0</m>.
                    </p>
                </statement>
                <proof>
                    <p>
                        If <m>(x_1, · · · , x_n)</m> solves <m>E_1 = f_1, E_2 = f_2</m> then it solves the first equation in <m>E_1 =
f_1, E_2 + aE_1 = f_2 + a f_1 </m>. Also, it satisfies <m> aE_1 = a f_1</m> and so, since it also solves <m>E_2 = f_2</m> it
must solve <m>E_2 + aE_1 = f_2 + a f_1 </m>. Therefore, if <m>(x_1, · · · , x_n )</m> solves <m>E_1 = f_1, E_2 = f_2</m> it must
also solve<m> E_2 + aE_1 = f_2 + a f_1</m>. On the other hand, if it solves the system <m>E_1 = f_1</m> and
<m>E_2 + aE_1 = f_2 + a f_1</m> , then <m>aE_1 = a f_1</m> and so you can subtract these equal quantities from
both sides of <m>E_2 +aE_1 = f_2 +a f_1</m> to obtain <m>E_2 = f_2</m> showing that it satisfies <m>E_1 = f_1 , E_2 = f_2</m> .</p>+
<p>The second assertion of the theorem which says that the system <m>E_1 = f_1 , E_2 = f_2</m> has the
same solution as the system, <m>E_2 = f_2 , E_1 = f_1</m> is seen to be true because it involves nothing
more than listing the two equations in a different order. They are the same equations.</p>

<p>The third assertion of the theorem which says <m>E_1 = f_1 , E_2 = f_2</m> has the same solution
as the system <m>E_1 = f_1, aE_2 = a f_2</m> provided <m>a\neq 0</m> is verified as follows: If <m>(x_1 , · · · , x_n )</m> is a
solution of <m>E_1 = f_1 , E_2 = f_2</m> , then it is a solution to <m>E_1 = f_1 , aE_2 = a f_2</m> because the second
system only involves multiplying the equation, <m>E_2 = f_2</m> by <m>a</m>. If <m>(x_1, · · · , x_n)</m> is a solution
of <m>E_1 = f_1 , aE_2 = a f_2</m>, then upon multiplying <m>aE_2 = a f_2</m> by the number <m>1/a</m>, you find that
<m>E_2 = f_2. \Box</m>
                    </p>
                </proof>
            </theorem>
            
	<p>
        Stated simply, the above theorem shows that the elementary operations do not change
the solution set of a system of equations.
    </p>
    <p>
        Here is an example in which there are three equations and three variables. You want to
find values for <m>x, y, z</m> such that each of the given equations are satisfied when these values
are plugged in to the equations.
    </p>
    <example xml:id="ex-elementary-operations">
        <statement>
            <p>
                Find the solutions to the system,
                <me>x + 3y + 6z = 25</me>
                <me>2x + 7y + 14z = 58</me>
                <me>2y + 5z = 19.</me>
            </p>
        </statement>
        <solution>
            <p>To solve this system replace the second equation by <m>(-2)</m> times the first equation added
to the second. This yields the system
<md>
    <mrow> x + 3y + 6z \amp = 25 </mrow>
    <mrow> y + 2z \amp = 8 </mrow>
    <mrow> 2y + 5z \amp = 19 </mrow>
</md>
Now take <m>(-2)</m> times the second and add to the third. More precisely, replace the third
equation with <m>(-2)</m> times the second added to the third. This yields the system
<md>
    <mrow> x + 3y + 6z \amp = 25 </mrow>
    <mrow> y + 2z \amp = 8 </mrow>
    <mrow> z \amp = 3 </mrow>
</md>
At this point, you can tell what the solution is. This system has the same solution as the
original system and in the above, <m>z = 3</m>. Then using this in the second equation, it follows
<m>y + 6 = 8</m> and so <m>y = 2</m>. Now using this in the top equation yields <m>x + 6 + 18 = 25</m> and so
<m>x = 1</m>. This process is called <term>back substitution</term>.</p>
    
<p>
Alternatively, you could have continued as follows. Add <m>(-2)</m> times the bottom
equation to the middle and then add <m>(-6)</m> times the bottom to the top. This yields
<me>x + 3y = 7, y = 2, z = 3</me>
Now add <m>(-3)</m> times the second to the top. This yields
<me>x = 1, y = 2, z = 3,</</me>
a system which has the same solution set as the original system. This avoided back substi-
tution and led to the same solution set.
            </p>
        </solution>
    </example>
	</subsection>

	<subsection xml:id="ss-gauss-elimination">
        <!-- <me>A = \left(
            \begin{array}{ccccc}
            a_{11} &amp; a_{12} &amp; a_{13} &amp; \cdots  &amp; a_{1n} \\
            a_{21} &amp; a_{22} &amp; a_{23} &amp; \cdots  &amp; a_{2n} \\
            a_{31} &amp; a_{32} &amp; a_{33} &amp; \cdots  &amp; a_{3n} \\
            \vdots  &amp; \vdots  &amp; \vdots  &amp; \ddots &amp; \vdots  \\
            a_{m1} &amp; a_{m2} &amp; a_{m3} &amp; \cdots  &amp; a_{mn} \\
            \end{array} \right)</me> -->
		<title>Gauss Elimination</title>
		<idx>Gauss Elimination</idx>
		<p>A less cumbersome way to represent a linear system is to write it as an <term>augmented matrix</term>.
            For example the linear system, 4.4 can be written as 
            <me>
				\left( \begin{array}{c c c | c}
				1 &amp; 3 &amp; 6 &amp; 25 \\
				2 &amp; 7 &amp; 14 &amp; 58 \\
				0 &amp; 2 &amp; 5 &amp; 19 \\
				\end{array} \right)
</me>
It has exactly the same
information as the original system but here it is understood there is an <m>x</m> column 
<m>
    \left( \begin{array}{c}
    1 \\
    2 \\
    0 \\
    \end{array} \right)
</m>, a <m>y</m> column, <m>
    \left( \begin{array}{c}
    3 \\
    7 \\
    2 \\
    \end{array} \right)
</m>, and a <m>z</m> column, 
<m>
    \left( \begin{array}{c}
    6 \\
    14 \\
    5 \\
    \end{array} \right)
</m>. The rows correspond to the equations in the system. Thus the top row in the augmented matrix corresponds
to the equation,
<me>x + 3y + 6z = 25</me>. Now when you replace an equation with a multiple of another equation added to itself, you
are just taking a row of this augmented matrix and replacing it with a multiple of another row added to it. 
        Thus the first step in solving <xref ref="ex-elementary-operations"/> would be to take <m>(-2)</m> times the first row
of the augmented matrix above and add it to the second row,
<me>
    \left( \begin{array}{c c c | c}
    1 &amp; 3 &amp; 6 &amp; 25 \\
    0 &amp; 1 &amp; 2 &amp; 8 \\
    0 &amp; 2 &amp; 5 &amp; 19 \\
    \end{array} \right)
</me>

<!-- STOPPED HERE p60 "Note how this corresponds to 4.5" in book is next line -->
		</p>

		<p>The top row and left column of an operation table are the column and row headings,
			respectively. To determine <m>a\oplus b</m>, find the entry in the row labeled <m>a</m>
			and the column labeled <m>b</m>. The following operation table serves to define * on <m>\{i,
			j, k\}</m>. <me>
				\begin{array}{c | c c c}
				* &amp; i &amp; j &amp; k \\ \hline
				i &amp; i &amp; i &amp; i \\
				j &amp; j &amp; j &amp; j \\
				k &amp; k &amp; k &amp; k
				\end{array}
</me>
		</p>
		<p>Note that <m>j*k = j</m>, yet <m>k * j = k</m>. Thus, <m>*</m> is not commutative.
			Commutativity is easy to identify in a table: the table must be symmetric with respect
			to the diagonal going from the top left to lower right.</p>

	</subsection>

	<exercises xml:id="exercises-11-1">
		<title>Exercises</title>
		<exercise number="1">
			<statement>
				<p> Determine the properties that the following operations have on the positive
					integers. <ol marker="(a)">
						<li>
							<p> addition</p>
						</li>
						<li>
							<p> multiplication</p>
						</li>
						<li>
							<p>
								<m>M</m> defined by <m>a M b = \textrm{ larger} \textrm{ of } a
					\textrm{ and } b</m></p>
						</li>
						<li>
							<p>
								<m>m</m> defined by <m>a m b = \textrm{ smaller} \textrm{ of } a
					\textrm{ and } b</m></p>
						</li>
						<li>
							<p>
								<m>@</m> defined by <m>a @ b = a^b</m></p>
						</li>
					</ol>
				</p>
			</statement>
			<answer>
				<p>
					<ol marker="(a)">
						<li>
							<p>Commutative, and associative. Notice that zero is the identity for
								addition, but it is not a positive integer.</p>
						</li>
						<li>
							<p> Commutative, associative, and has an identity (1)</p>
						</li>
						<li>
							<p> Commutative, associative, has an identity (1), and is idempotent</p>
						</li>
						<li>
							<p> Commutative, associative, and idempotent</p>
						</li>
						<li>
							<p> None. Notice that <m>2 @ (3 @ 3) = 512</m>, while <m>(2 @ 3) @ 3 =
								64</m>; and <m>a @ 1 = a</m>, while <m>1 @ a = 1</m>.</p>
						</li>
					</ol>
				</p>
			</answer>
		</exercise>
		<exercise number="2">
			<statement>
				<p>Which pairs of operations in Exercise 1 are distributive over one another?</p>
			</statement>
		</exercise>
		<exercise number="3">
			<statement>
				<p>Let <m>\bullet </m> be an operation on a set <m>S</m> and <m>A, B \subseteq S</m>.
					Prove that if <m>A</m> and <m>B</m> are both closed under <m>\bullet </m>, then <m>A\cap
					B</m> is also closed under <m>\bullet </m>, but <m>A \cup B</m> need not be.</p>
			</statement>
			<answer>
				<p>
					<me>
						\begin{split}
						a, b \in A \cap B &amp; \Rightarrow a, b \in A \textrm{ by the definition of
					intersection}\\
						&amp; \Rightarrow a\bullet b \in A\textrm{ by the closure of } A \textrm{
					with respect to } \bullet
						\end{split}
</me>
					Similarly, <m>a, b \in A \cap B \Rightarrow a\bullet b \in B</m>. Therefore, <m>a
					\bullet b \in A \cap B</m>. The set of positive integers is closed under
					addition, and so is the set of negative integers, but <m>1 + -1 - 0</m>.
					Therefore, their union, the nonzero integers, is not closed under addition.</p>
			</answer>
		</exercise>
		<exercise number="4">
			<statement>
				<p> How can you pick out the identity of an operation from its table?</p>
			</statement>
		</exercise>
		<exercise number="5">
			<statement>
				<p> Define <m>a \bullet b</m> by <m>\lvert a - b \rvert</m>, the absolute value of <m>a
					- b</m>. Which properties does <m>\bullet </m> have on the set of natural
					numbers, <m>\mathbb{N}</m>?</p>
			</statement>
			<answer>
				<p>
					<ol marker="(a)">
						<li>
							<p>
								<m>\bullet </m> is commutative since <m>\left| a-b\right| =\left|
								b-a\right|</m> for all <m>a, b \in \mathbb{N}</m></p>
						</li>
						<li>
							<p>
								<m>\bullet </m> is not associative. Take <m>a = 1</m>, <m>b = 2</m>,
								and <m>c = 3</m>, then <m>(a \bullet b) \bullet c =\left| \left|
								1-2\right| -3\right| =2</m> , and <m>a \bullet (b \bullet c) =
								\left| 1-\left| 2-3\right| \right| = 0</m>.</p>
						</li>
						<li>
							<p> Zero is the identity for <m>\bullet </m> on <m>\mathbb{N}</m>, since <m>a\bullet
								0=\left| a - 0\right| = a = \left| 0-a\right| = 0 \bullet a.</m></p>
						</li>
						<li>
							<p> Each element of <m>\mathbb{N}</m> inverts itself since <m>a \bullet
								a=\left| a-a\right| = 0</m>.</p>
						</li>
						<li>
							<p>
								<m>\bullet </m> is not idempotent, since, for <m>a\neq 0</m>, <m>a
								\bullet a =0 \neq a</m>.</p>
						</li>
					</ol>
				</p>
			</answer>
		</exercise>

	</exercises>
</section>
